olcoq/theories/OL_Reflection_4_fmap.v
@@ -216,6 +216,56 @@ Proof. compare_anterm_t. Qed.
 
 Require OrderedType OrderedTypeAlt.
 
+Definition compare_bool (x y: bool) : comparison :=
+  match x, y with
+  | true, true => Eq
+  | true, false => Gt
+  | false, true => Lt
+  | false, false => Eq
+  end.
+
+Lemma compare_bool_sym: forall x y: bool, compare_bool y x = CompOpp (compare_bool x y).
+Proof.
+  destruct x, y; simpl; congruence.
+Qed.
+
+Lemma compare_bool_trans: forall c x y z,
+    compare_bool x y = c ->
+    compare_bool y z = c ->
+    compare_bool x z = c.
+Proof.
+  destruct x, y, z; simpl; congruence.
+Qed.
+
+Lemma compare_bool_refl: forall x: bool, compare_bool x x = Eq.
+Proof. destruct x; simpl; auto. Qed.
+
+Lemma compare_bool_eq: forall x y: bool, compare_bool x y = Eq -> x = y.
+Proof.
+  destruct x, y; simpl; try congruence.
+Qed.
+
+Lemma compare_bool_eq_sym: forall x y: bool, compare_bool x y = Eq -> compare_bool y x = Eq.
+Proof. destruct x, y; simpl; congruence. Qed. 
+
+Lemma compare_bool_eq_trans: forall x y z: bool,
+    compare_bool x y = Eq ->
+    compare_bool y z = Eq ->
+    compare_bool x z = Eq.
+Proof. destruct x, y, z; simpl; congruence. Qed.
+
+Lemma compare_bool_antisym_impl: forall x y c, compare_bool x y = c -> compare_bool y x = CompOpp c.
+Proof. intros; destruct x, y, c; simpl in *; congruence. Qed.
+
+
+Module bool_as_OTA <: OrderedTypeAlt.OrderedTypeAlt.
+  Definition t := bool.
+  Definition compare := compare_bool.
+  Definition compare_sym := compare_bool_sym.
+  Definition compare_trans := compare_bool_trans.
+End bool_as_OTA.
+
+
 Module AnTerm_as_OTA <: OrderedTypeAlt.OrderedTypeAlt.
   Definition t := AnTerm.
   Definition compare := compare_anterm.
@@ -240,7 +290,7 @@ Module AnTerm_as_OT <: OrderedType.OrderedType.
 
   Theorem compare : forall x y : t, OrderedType.Compare lt eq x y.
   Proof.
-    intros x y; destruct (compare_anterm x y) eqn:Hcmp;
+    intros x y. destruct (compare_anterm x y) eqn:Hcmp;
       [ | | apply compare_anterm_antisym_impl in Hcmp; simpl in Hcmp ].
     all: econstructor; solve [unfold lt, eq; eassumption].
   Defined.
@@ -252,23 +302,53 @@ Module AnTerm_as_OT <: OrderedType.OrderedType.
   Defined.
 End AnTerm_as_OT.
 
-Require MSets MSetAVL MSetFacts.
 
+Module bool_as_OT <: OrderedType.OrderedType.
+  Definition t := bool.
+
+  Definition eq (x y: bool) := compare_bool x y = Eq.
+  Definition lt (x y: bool) := compare_bool x y = Lt.
+
+  Definition eq_refl : forall x : t, eq x x := compare_bool_refl.
+  Definition eq_sym : forall x y : t, eq x y -> eq y x := compare_bool_eq_sym.
+  Definition eq_trans : forall x y z : t, eq x y -> eq y z -> eq x z := compare_bool_eq_trans.
+  Definition lt_trans : forall x y z : t, lt x y -> lt y z -> lt x z := compare_bool_trans Lt.
+
+  Theorem lt_not_eq : forall x y : t, lt x y -> ~ eq x y.
+  Proof. unfold lt, eq; congruence. Qed.
+
+  Theorem compare : forall x y : t, OrderedType.Compare lt eq x y.
+  Proof. intros x y; destruct (compare_bool x y) eqn:Hcmp;
+      [ | | apply compare_bool_antisym_impl in Hcmp; simpl in Hcmp ].
+    all: econstructor; solve [unfold lt, eq; eassumption].
+  Defined.
+
+  Definition eq_dec : forall x y : t, {eq x y} + {~ eq x y}.
+  Proof.
+    intros x y; destruct (compare_bool x y) eqn:Hcmp; [ left | right.. ].
+    all: unfold eq; congruence.
+  Defined.
+End bool_as_OT.
+Require MSets MSetAVL MSetFacts.
+(*
 Module AnTerm_as_OOT := OrdersAlt.OT_from_Alt AnTerm_as_OTA.
 Module AnTermAVL := MSetAVL.Make AnTerm_as_OOT.
 Module AnTermPair_as_OOT := OrdersEx.PairOrderedType AnTerm_as_OOT AnTerm_as_OOT.
 Module AnTermPairAVL := MSetAVL.Make AnTermPair_as_OOT.
 Module AnTermPairAVLFacts := MSetFacts.Facts AnTermPairAVL.
-
+*)
 Require Import FMapAVL FMapFacts.
 Module AnTermPair_as_OT := OrderedTypeEx.PairOrderedType AnTerm_as_OT AnTerm_as_OT.
+Module AnTermPairBool_as_OT := OrderedTypeEx.PairOrderedType AnTermPair_as_OT bool_as_OT.
+Module AnTermPairBoolBool_as_OT := OrderedTypeEx.PairOrderedType AnTermPairBool_as_OT bool_as_OT.
+
 (* Module AnTermPair_as_OOT := OrdersAlt.Update_OT AnTermPair_as_OT. *)
 (* Module AnTermPairAVL := MSetAVL.Make AnTermPair_as_OOT. *)
-Module AnTermPairAVLMap := FMapAVL.Make AnTermPair_as_OT.
+Module AnTermPairAVLMap := FMapAVL.Make AnTermPairBoolBool_as_OT.
 Module AnTermPairAVLMapFacts := FMapFacts.Facts AnTermPairAVLMap.
 
 
-Definition MemoKey := (AnTerm * AnTerm)%type.
+Definition MemoKey := (AnTerm * AnTerm * bool * bool)%type.
 
 
 Definition MemoMap := AnTermPairAVLMap.t bool.
@@ -302,8 +382,8 @@ Module F := AnTermPairAVLMapFacts.
 (* Module Import M := AnTermPairAVL. *)
 (* Module Import F := AnTermPairAVLFacts. *)
 
-Fixpoint decideOL_fmap (fuel: nat) (g d: AnTerm) (memo: MemoMap) : (bool * MemoMap) :=
-  match M.find (g, d) memo with
+Fixpoint decideOL_fmap (fuel: nat) (g d: AnTerm) (cg cd: bool) (memo: MemoMap) : (bool * MemoMap) :=
+  match M.find (g, d, cg, cd) memo with
   | Some b => (b, memo)
   | None => (match fuel with
     | 0 => (false, memo) 
@@ -317,70 +397,76 @@ Fixpoint decideOL_fmap (fuel: nat) (g d: AnTerm) (memo: MemoMap) : (bool * MemoM
       | (R (Var a), N) => mfalse
       | (N, L (Var a)) => mfalse
       | (N, R (Var a)) => mfalse
-      | (L (Join a b), _) => decideOL_fmap n (L a) d &&& decideOL_fmap n (L b) d
-      | (_, L (Join a b)) => decideOL_fmap n g (L a) &&& decideOL_fmap n g (L b)
-      | (R (Meet a b), _) => decideOL_fmap n (R a) d &&& decideOL_fmap n (R b) d
-      | (_, R (Meet a b)) => decideOL_fmap n g (R a) &&& decideOL_fmap n g (R b)
-      | (L (Not a), _) => decideOL_fmap n (R a) d
-      | (_, L (Not a)) => decideOL_fmap n g (R a)
-      | (R (Not a), _) => decideOL_fmap n (L a) d
-      | (_, R (Not a)) => decideOL_fmap n g (L a)
+      | (L (Join a b), _) => decideOL_fmap n (L a) d false cd &&& decideOL_fmap n (L b) d false cd
+      | (_, L (Join a b)) => decideOL_fmap n g (L a) cg false &&& decideOL_fmap n g (L b) cg false
+      | (R (Meet a b), _) => decideOL_fmap n (R a) d false cd &&& decideOL_fmap n (R b) d false cd
+      | (_, R (Meet a b)) => decideOL_fmap n g (R a) cg false &&& decideOL_fmap n g (R b) cg false
+      | (L (Not a), _) => decideOL_fmap n (R a) d false cd
+      | (_, L (Not a)) => decideOL_fmap n g (R a) cg false
+      | (R (Not a), _) => decideOL_fmap n (L a) d false cd
+      | (_, R (Not a)) => decideOL_fmap n g (L a) cg false
       | _ => (
         match g with 
-        | L (Meet a b) => decideOL_fmap n (L a) d 
+        | L (Meet a b) => decideOL_fmap n (L a) d false cd 
         | _ => mfalse
         end ||| (
         match g with 
-        | L (Meet a b) => decideOL_fmap n (L b) d
+        | L (Meet a b) => decideOL_fmap n (L b) d false cd
         | _ => mfalse
         end ||| (
         match d with 
-        | L (Meet a b) => decideOL_fmap n g (L a) 
+        | L (Meet a b) => decideOL_fmap n g (L a) cg false 
         | _ => mfalse
         end ||| (
         match d with 
-        | L (Meet a b) => decideOL_fmap n g (L b) 
+        | L (Meet a b) => decideOL_fmap n g (L b) cg false 
         | _ => mfalse
         end ||| (
         match g with
-        | R (Join a b) => decideOL_fmap n (R a) d
+        | R (Join a b) => decideOL_fmap n (R a) d false cd
         | _ => mfalse
         end ||| (
         match g with
-        | R (Join a b) => decideOL_fmap n (R b) d
+        | R (Join a b) => decideOL_fmap n (R b) d false cd
         | _ => mfalse
         end ||| (
         match d with
-        | R (Join a b) => decideOL_fmap n g (R a) 
+        | R (Join a b) => decideOL_fmap n g (R a) cg false 
         | _ => mfalse
         end ||| (
         match d with
-        | R (Join a b) => decideOL_fmap n g (R b)
+        | R (Join a b) => decideOL_fmap n g (R b) cg false
         | _ => mfalse
         end ||| (
-        match d with 
-        | N => decideOL_fmap n g g 
+        match (d, cg) with 
+        | (N, false) => decideOL_fmap n g g true true 
         | _ => mfalse
         end ||| (
-        match g with 
-        | N => decideOL_fmap n d d
+        match (g, cd) with 
+        | (N, false) => decideOL_fmap n d d true true
         | _ => mfalse
         end  ||| (
-        decideOL_fmap n g N ||| 
-        decideOL_fmap n N d
-        )))))))))))
-      end) (AnTermPairAVLMap.add (g, d) false memo)
-    in (b, AnTermPairAVLMap.add (g, d) b m) end)
+        match d with 
+        | N => mfalse
+        | _ => decideOL_fmap n g N cg true
+        end ||| (
+        match g with
+        | N => mfalse
+        | _ => decideOL_fmap n N d true cd
+        end
+        ))))))))))))
+      end) memo
+    in (b, AnTermPairAVLMap.add (g, d, cg, cd) b m) end)
 end.
 
 
 Definition decideOL_fmap_simp (g d: AnTerm): bool :=
-  fst (decideOL_fmap ((anterm_size g * anterm_size d) + 4) g d (AnTermPairAVLMap.empty bool)).
+  fst (decideOL_fmap ((anterm_size g * anterm_size d) + 4) g d false false (AnTermPairAVLMap.empty bool)).
 
 
-Definition memomap_correct (l: MemoMap) :=  forall g d, 
-  match M.find (g, d) l with
-  | Some true => exists n,  (decideOL_opti n g d = true)
+Definition memomap_correct (l: MemoMap) :=  forall g d cg cd, 
+  match M.find (g, d, cg, cd) l with
+  | Some true => exists n,  (decideOL_opti n g d cg cd = true)
   | _ => True
   end.
 
@@ -458,13 +544,13 @@ Proof.
 Qed.
 
 
-Lemma memomap_correct_cons g d l e : 
+Lemma memomap_correct_cons g d cg cd l e : 
   memomap_correct l /\
-  (e = true -> exists n, decideOL_opti n g d = true) -> 
-  memomap_correct (AnTermPairAVLMap.add (g, d) e l) /\ (e = true -> exists n, decideOL_opti n g d = true).
+  (e = true -> exists n, decideOL_opti n g d cg cd = true) -> 
+  memomap_correct (AnTermPairAVLMap.add (g, d, cg, cd) e l) /\ (e = true -> exists n, decideOL_opti n g d cg cd = true).
 Proof.
   unfold memomap_correct; intro H1; destruct H1 as [Hok He]. split; auto. intros.
-  rewrite F.add_o; destruct F.eq_dec as [(Heq1%compare_anterm_eq, Heq2%compare_anterm_eq) | Hneq ].
+  rewrite F.add_o; simpl in *; destruct F.eq_dec as [(((Heq1%compare_anterm_eq, Heq2%compare_anterm_eq), Heq3%compare_bool_eq), Heq4%compare_bool_eq) | Hneq ].
   - destruct e; auto. simpl in *; subst; apply He, reflexivity.
   - simpl in *. apply Hok.
 Qed.
@@ -479,29 +565,29 @@ Proof.
 Qed.
 
 
-Lemma memomap_correct_false g d l: memomap_correct l -> memomap_correct ( AnTermPairAVLMap.add (g, d) false l).
+Lemma memomap_correct_false g d cg cd l: memomap_correct l -> memomap_correct ( AnTermPairAVLMap.add (g, d, cg, cd) false l).
 Proof.
-  intros. unfold memomap_correct. intros. rewrite F.add_o; destruct F.eq_dec as [(Heq1%compare_anterm_eq, Heq2%compare_anterm_eq) | Hneq ]; auto.
+  intros. unfold memomap_correct. intros. rewrite F.add_o; destruct F.eq_dec as [(((Heq1%compare_anterm_eq, Heq2%compare_anterm_eq), Heq3%compare_bool_eq), Heq4%compare_bool_eq) | Hneq ]; auto.
   simpl in *. apply H.
 Qed.
 
 
 Theorem decideOL_fmap_correct : 
-  forall n g d l, 
+  forall n g d cg cd l, 
   (memomap_correct l) -> 
-  (memomap_correct (snd (decideOL_fmap n g d l))) /\
-  (((fst (decideOL_fmap n g d l)) = true) ->  exists n0, (decideOL_opti n0 g d) = true).
+  (memomap_correct (snd (decideOL_fmap n g d cg cd l))) /\
+  (((fst (decideOL_fmap n g d cg cd l)) = true) ->  exists n0, (decideOL_opti n0 g d cg cd) = true).
 Proof.
     induction n.
   - intros. split.
-    + intros. pose proof (H g d). simpl in *. destruct M.find; simpl in *; auto.
-    + specialize (H g d). simpl in *.
+    + intros. pose proof (H g d cg cd). simpl in *. destruct M.find; simpl in *; auto.
+    + specialize (H g d cg cd). simpl in *.
       destruct M.find; intros; simpl in *; subst; congruence.
   - intros.
-    + simpl. pose proof H. unfold memomap_correct in H0.  specialize (H0 g d).
+    + simpl. pose proof H. unfold memomap_correct in H0.  specialize (H0 g d cg cd).
       destruct M.find eqn: res. simpl in *. destruct b; simpl in *; auto. split; auto; intro; congruence.
 
-      pose proof (memomap_correct_false g d l H) as H1. 
+      pose proof (memomap_correct_false g d cg cd l H) as H1. 
       dest_simp g; dest_simp d; (try dest_simp t0); (try dest_simp t). all: repeat rewrite mor_mtrue_r; repeat rewrite mor_mfalse_l; repeat rewrite mand_mtrue_l.
 
       all: rewrite snd_let_simpl; rewrite fst_let_simpl. all: repeat rewrite mor_mtrue_r; repeat rewrite mor_mfalse_l; repeat rewrite mand_mtrue_l.
@@ -516,9 +602,9 @@ Proof.
         let IHn_fst := (fresh "IHn_fst") in let n0 := (fresh "n0") in 
         let b_ := (fresh "b") in let l_ := (fresh "l") in let found := (fresh "found") in
           lazymatch rest with
-          | decideOL_fmap ?n ?g ?d => 
-            pose proof (IHn g d l H) as IHn_; simpl in *; destruct IHn_ as [IHn_snd IHn_fst];
-            destruct (decideOL_fmap n g d l) as [b_ l_] eqn: found;
+          | decideOL_fmap ?n ?g ?d ?cg ?cd => 
+            pose proof (IHn g d cg cd l H) as IHn_; simpl in *; destruct IHn_ as [IHn_snd IHn_fst];
+            destruct (decideOL_fmap n g d cg cd l) as [b_ l_] eqn: found;
             destruct b_; simpl in *;
             only 1: (destruct IHn_fst as [n0 IHn_fst]; auto; simpl in *;
               split; auto; intro; exists (S n0); simpl; 
@@ -526,10 +612,10 @@ Proof.
             split; auto; congruence;
             idtac
 
-          | decideOL_fmap ?n ?g ?d ||| ?rest2 =>
-            try rewrite_mor (decideOL_fmap n g d) rest2 l;
-            pose proof (IHn g d l H) as IHn_; simpl in *; destruct IHn_ as [IHn_snd IHn_fst];
-            destruct (decideOL_fmap n g d l) as [b_ l_] eqn: found;
+          | decideOL_fmap ?n ?g ?d ?cg ?cd ||| ?rest2 =>
+            try rewrite_mor (decideOL_fmap n g d cg cd) rest2 l;
+            pose proof (IHn g d cg cd l H) as IHn_; simpl in *; destruct IHn_ as [IHn_snd IHn_fst];
+            destruct (decideOL_fmap n g d cg cd l) as [b_ l_] eqn: found;
             destruct b_; simpl in *;
             only 1: (destruct IHn_fst as [n0 IHn_fst]; auto; simpl in *;
               split; auto; intro; exists (S n0); simpl; 
@@ -537,15 +623,15 @@ Proof.
             reduce_or rest2 IHn l_ IHn_snd;
             idtac
 
-          | (decideOL_fmap ?n ?g1 ?d1) &&& (decideOL_fmap ?n ?g2 ?d2)  =>
-            try rewrite_mand (decideOL_fmap n g1 d1) (decideOL_fmap n g2 d2) l;
+          | (decideOL_fmap ?n ?g1 ?d1 ?cg1 ?cd1) &&& (decideOL_fmap ?n ?g2 ?d2 ?cg2 ?cd2)  =>
+            try rewrite_mand (decideOL_fmap n g1 d1 cg1 cd1) (decideOL_fmap n g2 d2 cg2 cd2) l;
             let IHn_snd_r := (fresh "IHn_snd_r") in let IHn_fst_r := (fresh "IHn_fst_r") in
             let IHn_r := (fresh "IHn_r") in let m1 := (fresh "m1") in let m2 := (fresh "m2") in
             let b_r := (fresh "b_r") in let l_r := (fresh "l_r") in let found_r := (fresh "found_r") in
-            pose proof (IHn g1 d1 l H) as IHn_; simpl in *; destruct IHn_ as [IHn_snd IHn_fst];
-            destruct (decideOL_fmap n g1 d1 l)  as [ b_ l_] eqn: found;
-            pose proof (IHn g2 d2 l_ IHn_snd) as IHn_r; simpl in *; destruct IHn_r as [IHn_snd_r IHn_fst_r];
-            destruct (decideOL_fmap n g2 d2 l_)  as [ b_r l_r] eqn: found_r;
+            pose proof (IHn g1 d1 cg1 cd1 l H) as IHn_; simpl in *; destruct IHn_ as [IHn_snd IHn_fst];
+            destruct (decideOL_fmap n g1 d1 cg1 cd1 l)  as [ b_ l_] eqn: found;
+            pose proof (IHn g2 d2 cg2 cd2 l_ IHn_snd) as IHn_r; simpl in *; destruct IHn_r as [IHn_snd_r IHn_fst_r];
+            destruct (decideOL_fmap n g2 d2 cg2 cd2 l_)  as [ b_r l_r] eqn: found_r;
             simpl in *;
             destruct b_ ; destruct b_r ; simpl in *;
             only 1: (destruct IHn_fst as [m1 IHn_fst]; destruct IHn_fst_r as [m2 IHn_fst_r]; auto;
@@ -568,20 +654,28 @@ Proof.
             idtac
       end.
       all: try (lazymatch goal with
-      | [ |- memomap_correct (_ (?g, ?d) (fst (?rest ?l)) (snd (?rest ?l))) /\ _ ] => 
+      | [ |- memomap_correct (_ (?g, ?d, ?cg, ?cd) (fst (?rest ?l)) (snd (?rest ?l))) /\ _ ] => 
         apply memomap_correct_cons;
-        reduce_or rest IHn l H1;
+        reduce_or rest IHn l H;
         idtac
       | _ => fail "unknown shape"
       end; fail). 
+      all: destruct cg; destruct cd; repeat rewrite mor_mfalse_l.
+      all: lazymatch goal with
+      | [ |- memomap_correct (_ (?g, ?d, ?cg, ?cd) (fst (?rest ?l)) (snd (?rest ?l))) /\ _ ] => 
+        apply memomap_correct_cons;
+        reduce_or rest IHn l H;
+        idtac
+      | _ => fail "unknown shape"
+      end.
 Qed.
 
 
 Theorem decideOL_fmap_simp_correct : forall g d, (decideOL_fmap_simp g d) = true -> anTerm_leq g d.
 Proof. 
   intros. assert (squash (OLProof (g, d))). 
-  pose proof (decideOL_fmap_correct (anterm_size g * anterm_size d + 4) g d (AnTermPairAVLMap.empty bool)). 
-  destruct H0. unfold memomap_correct; simpl in *; auto. destruct H1 as [n0 H1]; auto. apply decideOL_opti_correct with n0; auto.
+  pose proof (decideOL_fmap_correct (anterm_size g * anterm_size d + 4) g d false false (AnTermPairAVLMap.empty bool)). 
+  destruct H0. unfold memomap_correct; simpl in *; auto. destruct H1 as [n0 H1]; auto. apply decideOL_opti_correct with n0 false false; auto.
   destruct H0. apply (soundness (g, d)). auto.
 Qed.
 
